code/poly1305/Hacl.Impl.Poly1305.fsti
@@ -29,14 +29,22 @@ val state_inv_t: #s:field_spec -> h:mem -> ctx:poly1305_ctx s -> Type0
 
 
 // If the ctx is not modified, all the components and invariants are preserved
-val reveal_ctx_inv: #s:field_spec -> ctx:poly1305_ctx s -> h0:mem -> h1:mem ->
+val reveal_ctx_inv': #s:field_spec -> ctx:poly1305_ctx s -> ctx':poly1305_ctx s -> h0:mem -> h1:mem ->
   Lemma
+  (requires Seq.equal (as_seq h0 ctx) (as_seq h1 ctx') /\ state_inv_t h0 ctx)
+  (ensures
+    as_get_r h0 ctx == as_get_r h1 ctx' /\
+    as_get_acc h0 ctx == as_get_acc h1 ctx' /\
+    state_inv_t h1 ctx')
+
+let reveal_ctx_inv #s ctx h0 h1: Lemma
   (requires Seq.equal (as_seq h0 ctx) (as_seq h1 ctx) /\ state_inv_t h0 ctx)
   (ensures
     as_get_r h0 ctx == as_get_r h1 ctx /\
     as_get_acc h0 ctx == as_get_acc h1 ctx /\
     state_inv_t h1 ctx)
-
+=
+  reveal_ctx_inv' #s ctx ctx h0 h1
 
 inline_for_extraction noextract
 let poly1305_init_st (s:field_spec) =
