code/streaming/Hacl.Streaming.Poly1305_32.fst
@@ -1,0 +1,153 @@
+module Hacl.Streaming.Poly1305_32
+
+module HS = FStar.HyperStack
+module B = LowStar.Buffer
+module G = FStar.Ghost
+module S = FStar.Seq
+module U32 = FStar.UInt32
+module U64 = FStar.UInt64
+//module F = Hacl.Streaming.Functor
+module I = Hacl.Streaming.Interface
+module P = Hacl.Impl.Poly1305
+module F32xN = Hacl.Spec.Poly1305.Field32xN
+module ST = FStar.HyperStack.ST
+
+open LowStar.BufferOps
+open FStar.Mul
+
+/// Opening a bunch of modules for Poly1305
+
+inline_for_extraction noextract
+let uint8 = Lib.IntTypes.uint8
+
+inline_for_extraction noextract
+let uint32 = Lib.IntTypes.uint32
+
+open Hacl.Impl.Poly1305.Fields
+
+#set-options "--max_fuel 0 --max_ifuel 0 --z3rlimit 100"
+
+inline_for_extraction noextract
+let t = b:B.buffer (limb M32) { B.length b == 25 }
+
+inline_for_extraction noextract
+let as_raw (x: t): B.buffer (limb M32) = x
+
+inline_for_extraction noextract
+let as_lib (x: t): P.poly1305_ctx M32 =
+  assert_norm (Lib.IntTypes.(v (add #U32 (nlimb M32) (precomplen M32))) == 25);
+  x
+
+inline_for_extraction noextract
+let stateful_poly1305_ctx32: I.stateful unit =
+  I.Stateful
+    (fun () -> t)
+    (fun #_ _ s -> B.loc_addr_of_buffer (as_raw s))
+    (fun #_ _ s -> B.freeable (as_raw s))
+    (fun #_ h s -> B.live h (as_raw s) /\ P.state_inv_t h (as_lib s))
+    (fun () -> Spec.Poly1305.felem & Spec.Poly1305.felem)
+    (fun () h s -> P.as_get_acc h (as_lib s), P.as_get_r h (as_lib s))
+    (fun #_ _ _ -> ())
+    (fun #_ l s h0 h1 ->
+      P.reveal_ctx_inv (as_lib s) h0 h1;
+      B.modifies_buffer_elim (as_raw s) l h0 h1)
+    (fun #_ _ _ _ _ -> ())
+
+let update (acc, r) (block: S.seq uint8 { S.length block = Spec.Poly1305.size_block }) =
+  Spec.Poly1305.poly1305_update1 r Spec.Poly1305.size_block block acc, r
+
+inline_for_extraction noextract
+let k = I.stateful_buffer uint8 32
+
+inline_for_extraction noextract
+let as_lib_k (x: B.buffer uint8 { B.length x = 32 }): Lib.Buffer.lbuffer uint8 32ul =
+  x
+
+inline_for_extraction noextract
+let poly1305_32: I.block unit =
+  I.Block
+    I.Runtime
+
+    stateful_poly1305_ctx32
+    k
+
+    (fun () -> pow2 32 - 1)
+    (fun () -> 16ul)
+    (fun () -> 16ul)
+
+    (fun () k -> Spec.Poly1305.poly1305_init k)
+    (fun () acc blocks -> Spec.UpdateMulti.mk_update_multi Spec.Poly1305.size_block update acc blocks)
+    (fun () (acc, r) _ input -> Spec.Poly1305.poly1305_update1 r (S.length input) input acc, r)
+    (fun () k (acc, r) -> Spec.Poly1305.poly1305_finish k acc)
+
+    (fun () k input -> Spec.Poly1305.poly1305_mac input k)
+
+    (fun () -> Spec.UpdateMulti.update_multi_zero Spec.Poly1305.size_block update)
+    (fun () -> Spec.UpdateMulti.update_multi_associative Spec.Poly1305.size_block update)
+    (fun () _ _ -> admit ())
+
+    (fun _ _ -> ())
+    (fun () ->
+      let h0 = ST.get () in
+      let dummy_key = B.alloca (Lib.IntTypes.u8 0) 32ul in
+      let r = B.alloca (F32xN.zero 1) 25ul in
+      P.poly1305_init #M32 (as_lib r) (as_lib_k dummy_key);
+      let h1 = ST.get () in
+      B.modifies_only_not_unused_in B.loc_none h0 h1;
+      r)
+    (fun () r ->
+      let h0 = ST.get () in
+      ST.push_frame ();
+      let h1 = ST.get () in
+      let dummy_key = B.alloca (Lib.IntTypes.u8 0) 32ul in
+      let h11 = ST.get () in
+      let r = B.malloc r (F32xN.zero 1) 25ul in
+      let h12 = ST.get () in
+      P.poly1305_init #M32 (as_lib r) (as_lib_k dummy_key);
+      let h2 = ST.get () in
+      B.modifies_only_not_unused_in B.loc_none h1 h11;
+      B.modifies_only_not_unused_in B.loc_none h11 h12;
+      B.modifies_only_not_unused_in B.(loc_buffer r) h12 h12;
+      ST.pop_frame ();
+      let h3 = ST.get () in
+      B.modifies_fresh_frame_popped h0 h1 B.(loc_buffer r) h2 h3;
+      B.modifies_only_not_unused_in B.loc_none h0 h3;
+      P.reveal_ctx_inv (as_lib r) h2 h3;
+      r)
+    (fun _ k s -> P.poly1305_init #M32 s k)
+    (fun _ s blocks len -> P.poly1305_update #M32 s len blocks; admit ())
+    (fun _ s last total_len ->
+      admit ();
+      let len = FStar.Int.Cast.Full.uint64_to_uint32 (total_len `U64.rem` 16UL) in
+      P.poly1305_update #M32 s len last)
+    (fun _ k s dst ->
+      let h0 = ST.get () in
+      ST.push_frame ();
+      let h1 = ST.get () in
+      let tmp = B.alloca (F32xN.zero 1) 25ul in
+      let h2 = ST.get () in
+      B.modifies_only_not_unused_in B.loc_none h1 h2;
+      B.blit s 0ul tmp 0ul 25ul;
+      let h3 = ST.get () in
+      B.modifies_only_not_unused_in B.loc_none h1 h3;
+      P.reveal_ctx_inv' (as_lib s) (as_lib tmp) h0 h3;
+      P.poly1305_finish #M32 dst k tmp;
+      let h4 = ST.get () in
+      ST.pop_frame ();
+      let h5 = ST.get () in
+      B.modifies_only_not_unused_in B.(loc_buffer dst) h1 h4;
+      B.modifies_fresh_frame_popped h0 h1 B.(loc_buffer dst) h4 h5;
+      assert B.(loc_disjoint (loc_buffer s) (loc_buffer dst));
+      P.reveal_ctx_inv (as_lib s) h0 h5
+    )
+    (fun _ s -> B.free s)
+    (fun _ src dst ->
+      let h0 = ST.get () in
+      B.blit src 0ul dst 0ul 25ul;
+      let h1 = ST.get () in
+      P.reveal_ctx_inv' (as_lib src) (as_lib dst) h0 h1
+    )
+
+// Make sure SHA256 update last works
+// Update functor to deal with key
+// Do proof of spec equivalence lemma
